shiftreset/TriplesBindIndexed.v
@@ -1,0 +1,604 @@
+
+From ShiftReset Require Import LogicBind.
+Local Open Scope string_scope.
+
+Inductive eresult : Type :=
+  | enorm : val -> eresult
+  | eshft : (var -> expr) -> (val -> expr) -> eresult.
+
+Notation "'eshft(' k ',' eb ',' x ',' ek ')'" :=
+  (eshft k eb x ek) (at level 30, only printing,
+  format "'eshft(' k ','  eb ','  x ','  ek ')'" ).
+
+Definition penv := Fmap.fmap var (val -> expr).
+Implicit Types p penv : penv.
+
+#[global]
+Instance Inhab_pfun : Inhab (val -> expr).
+Proof.
+  constructor.
+  exists (fun a:val => pval vunit).
+  constructor.
+Qed.
+
+Definition empty_penv : penv := Fmap.empty.
+
+Coercion pval : val >-> expr.
+Coercion pvar : var >-> expr.
+Coercion vint : Z >-> val.
+
+Inductive bigstep : penv -> heap -> expr -> heap -> eresult -> Prop :=
+
+  | eval_pval : forall p1 h v,
+    bigstep p1 h (pval v) h (enorm v)
+
+  | eval_pfun : forall p h x e,
+    bigstep p h (pfun x e) h (enorm (vfun x e))
+
+  | eval_padd : forall p1 h v1 v2 i1 i2,
+    vint i1 = v1 ->
+    vint i2 = v2 ->
+    bigstep p1 h (padd (pval v1) (pval v2)) h (enorm (vint (i1 + i2)))
+
+  | eval_pshift : forall h p (eb:var->expr),
+    bigstep p h (pshift eb) h (eshft eb (fun v => pval v))
+
+  | eval_plet : forall p1 h1 h3 h2 x e1 e2 v Re,
+    bigstep p1 h1 e1 h3 (enorm v) ->
+    bigstep p1 h3 (subst x v e2) h2 Re ->
+    bigstep p1 h1 (plet x e1 e2) h2 Re
+
+  | eval_plet_sh : forall x e1 e2 h1 h2 p1 (eb:var->expr) (ek:val->expr),
+    bigstep p1 h1 e1 h2 (eshft eb ek) ->
+    bigstep p1 h1 (plet x e1 e2) h2 (eshft eb (fun y => plet x (ek y) e2))
+
+  | eval_papp_fun : forall v1 v2 h x e Re p1,
+    v1 = vfun x e ->
+    bigstep p1 h (subst x v2 e) h Re ->
+    bigstep p1 h (papp (pval v1) (pval v2)) h Re
+
+  (* | eval_app_fix : forall v1 v2 h x e Re xf p,
+    v1 = vfix xf x e ->
+    bigstep p h (subst x v2 (subst xf v1 e)) h Re ->
+    bigstep p h (papp (pval v1) (pval v2)) h Re *)
+
+  | eval_papp_unk : forall v h1 h2 Re (ef:val->expr) (f:var) p1,
+    Fmap.read p1 f = ef ->
+    bigstep p1 h1 (ef v) h2 Re ->
+    bigstep p1 h1 (papp (pvar f) (pval v)) h2 Re
+
+  | eval_preset_val : forall p1 h1 h2 p e v,
+    bigstep p1 h1 e h2 (enorm v) ->
+    bigstep p1 h1 (preset e) h2 (enorm v)
+
+  | eval_preset_sh : forall k p1 h1 h2 h3 e (eb:var->expr) (ek:val->expr) Re,
+    bigstep p1 h1 e h3 (eshft eb ek) ->
+    bigstep (Fmap.update p1 k ek) h3 (eb k) h2 Re ->
+    bigstep p1 h1 (preset e) h2 Re
+
+  .
+
+
+Module BigStepExamples.
+
+Example e1_shift : exists Re,
+  bigstep empty_penv empty_heap (pshift (fun k => pval (vint 1)))
+    empty_heap Re.
+Proof.
+  intros. eexists.
+  applys eval_pshift.
+  (* Show Proof. *)
+Qed.
+
+Example e2_shift_reset : forall (k1:var), exists Re,
+  bigstep empty_penv empty_heap (preset (pshift (fun k => papp k (pval (vint 1)))))
+    empty_heap Re.
+Proof.
+  intros. eexists.
+  applys eval_preset_sh k1.
+  applys eval_pshift.
+  simpl.
+  applys eval_papp_unk. reflexivity.
+  rewrite fmap_read_update.
+  applys eval_pval.
+  (* Show Proof. *)
+Qed.
+
+(* < let x1 = shift k. k in x1 + 1 > 1 *)
+Example e3_shift_k_k : forall (k:var), exists Re,
+  bigstep empty_penv empty_heap
+    (plet "x2"
+      (preset (plet "x1"
+        (pshift (fun k => pfun "x" (papp k (pvar "x"))))
+        (padd 1 (pvar "x1"))))
+      (papp (pvar "x2") 1))
+    empty_heap Re.
+Proof.
+  intros. eexists.
+  applys eval_plet.
+  { applys eval_preset_sh k.
+    (* we have to name the binders of the new functions created *)
+    { applys eval_plet_sh. applys_eq eval_pshift. }
+    { simpl. applys eval_pfun. } }
+  { simpl.
+    applys eval_papp_fun. reflexivity. simpl.
+Abort.
+(* we cannot handle dynamic continuations in triples without a simulation relation *)
+    (* applys eval_papp_fun. reflexivity. simpl.
+    applys eval_plet.
+    { applys eval_papp_fun. reflexivity. simpl.
+      applys eval_pval. }
+    simpl.
+    applys* eval_padd.
+  }
+  (* Show Proof. *)
+Qed. *)
+
+End BigStepExamples.
+
+Notation " '[' p1 ','  h1  '|'  e ']'  '~~>'  '[' p2 ','  h2  '|'  Re ']'" :=
+  (bigstep p1 h1 e p2 h2 Re) (at level 30, only printing).
+
+Notation "'pshift' k '.' e" :=
+  (pshift k e) (at level 30, only printing,
+  format "'pshift'  k '.'  e" ).
+
+
+Inductive spec_assert_valid_under penv (env:senv) : int -> expr -> flow -> Prop :=
+  | sav_base: forall e f,
+    (forall h1 h2 (eb:var->expr) (ek:val->expr),
+        not (bigstep penv h1 e h2 (eshft eb ek))) ->
+    (forall h1 h2 v,
+        bigstep penv h1 e h2 (enorm v) ->
+        satisfies env env h1 h2 (norm v) f) ->
+    spec_assert_valid_under penv env 0 e f
+
+| sav_shift: forall n e f, n > 0 ->
+    (forall h1 h2 v, not (bigstep penv h1 e h2 (enorm v))) ->
+    (forall h1 h2 (eb:var->expr) (ek:val->expr),
+        bigstep penv h1 e h2 (eshft eb ek) -> (* get the n from here? *)
+        exists (fb:var->flow) (fk:val->flow),
+          satisfies env env h1 h2 (shft fb fk) f /\
+            (forall x, spec_assert_valid_under penv env (n-1) (eb x) (fb x)) /\
+            (forall v, spec_assert_valid_under penv env (n-1) (ek v) (fk v))) ->
+    spec_assert_valid_under penv env n e f.
+
+(* Check spec_assert_valid_under_ind. *)
+(* Lemma spec_assert_valid_under_ind1 :
+  forall penv env (P:expr->flow->Prop),
+    (forall e f,
+      (forall h1 h2 eb ek, ~ bigstep penv h1 e h2 (eshft eb ek)) ->
+      (forall h1 h2 v,
+        bigstep penv h1 e h2 (enorm v) ->
+        satisfies env env h1 h2 (norm v) f) ->
+      P e f) ->
+    (forall e f,
+      (forall h1 h2 v, ~ bigstep penv h1 e h2 (enorm v)) ->
+      (forall h1 h2 eb ek,
+        bigstep penv h1 e h2 (eshft eb ek) ->
+        exists fb fk, satisfies env env h1 h2 (shft fb fk) f /\
+        (forall x, P (eb x) (fb x) -> spec_assert_valid_under penv env (eb x) (fb x)) /\
+        (forall v, P (ek v) (fk v) -> spec_assert_valid_under penv env (ek v) (fk v))) ->
+      P e f) ->
+    forall e f,
+      spec_assert_valid_under penv env e f -> P e f.
+Proof.
+  intros.
+  specializes H e f.
+  specializes H0 e f.
+  induction H1.
+  - clear H0. specializes H H1 H2.
+  - clear H. specializes H0 H1.
+    applys H0. clear H0.
+    intros.
+    specializes H2 H.
+    destr H2.
+    exists fb fk. splits*.
+Qed. *)
+
+Definition spec_assert_valid n e f : Prop :=
+  forall penv env,
+    spec_assert_valid_under penv env n e f.
+
+
+Lemma pval_sound: forall v,
+  spec_assert_valid 0 (pval v) (ens (fun r => \[r = v])).
+Proof.
+  unfold spec_assert_valid. intros.
+  applys sav_base. { introv H. false_invert H. }
+  introv H.
+  inverts H.
+  applys s_ens.
+  exs. intuition. hintro. reflexivity.
+  fmap_eq.
+Qed.
+
+Lemma pshift_sound: forall eb fb,
+  (forall n k, spec_assert_valid n (eb k) (fb k)) ->
+  spec_assert_valid 1 (pshift eb) (sh fb).
+Proof.
+  unfold spec_assert_valid. intros * Heb **.
+  applys sav_shift. math. { introv H. false_invert H. } intros.
+  inverts H.
+  exs.
+  splits.
+  { applys s_sh. }
+  { intros x. specializes Heb x penv0 env. }
+  { intros v. simpl. applys pval_sound. }
+Qed.
+
+Lemma papp_unk_sound: forall penv (env:senv) (f:var) v (ef:val->expr) (f1:val->flow) n,
+  Fmap.read penv f = ef ->
+  Fmap.read env f = f1 ->
+  spec_assert_valid_under penv env n (ef v) (f1 v) ->
+  spec_assert_valid_under penv env n (papp f v) (unk f v).
+Proof.
+  unfold spec_assert_valid. intros * ? ? He.
+  inverts He as.
+  { introv Hne He.
+    applys sav_base.
+    { introv H1. inverts H1 as H1 H2. rewrite H in H1. false Hne H1. }
+    intros * Hb.
+    inverts Hb as. intros Hb.
+    rewrite H in Hb.
+    specializes He Hb.
+    applys s_unk.
+    eassumption.
+    assumption. }
+  { intros * Hn Hne He.
+    applys sav_shift. math.
+    { introv H1. inverts H1 as H1 H2. rewrite H in H1. false Hne H1. }
+    intros * Hb.
+    inverts Hb as H3 H4.
+    rewrite H in H3.
+    specializes He H3. destruct He as (fk&fb&rb&?&?).
+    exs.
+    split*.
+    applys s_unk.
+    eassumption.
+    assumption. }
+Qed.
+
+
+Lemma papp_sound: forall x e (v:val) f n,
+  spec_assert_valid n (subst x v e) f ->
+  spec_assert_valid n (papp (vfun x e) v) f.
+Proof.
+  unfold spec_assert_valid.
+  intros * He penv env.
+  specializes He penv env.
+  inverts He as.
+  { introv Hne He.
+    (* no shift in the body of the fn being applied *)
+    applys sav_base.
+    { intros * H. inverts H as H H1. injects H. false Hne H1. }
+    intros.
+    inverts H as H H1. injects H.
+    specializes He H1.
+    assumption. }
+  { intros * Hn Hne He.
+    (* shift *)
+    applys sav_shift. math.
+    { introv H.
+      inverts H as H H1. injects H.
+      false Hne H1. }
+    intros.
+    inverts H as H H1. injects H.
+    specializes He H1. destr He.
+    exs.
+    splits*.
+  }
+Qed.
+
+Lemma plet_sound: forall n n1 x e1 e2 f1 (f2:val->flow),
+  spec_assert_valid n1 e1 f1 ->
+  n >= n1 ->
+  (forall v, spec_assert_valid (n-n1) (subst x v e2) (f2 v)) ->
+  spec_assert_valid n (plet x e1 e2) (bind f1 f2).
+Proof.
+  intros n.
+  induction_wf IH: (downto 0) n.
+  unfold spec_assert_valid in *.
+  introv He1 Hwf He2. intros. specializes He1 penv0 env.
+  inverts He1 as.
+  {
+    (* e1 has no shift *)
+    introv Hne1 Hb1.
+
+    (* if i am able to predict, this is all good *)
+    (* applys sav_shift.
+    admit. *)
+    (* intros.
+    inverts H.
+    { specializes He2 v penv0 env.
+    inverts He2. { false H H8. }
+    specializes H0 H8.
+    destr H0. exists fb fk.
+    splits*.
+    applys s_bind.
+    specializes Hb1 H7. eassumption.
+    assumption.
+    }
+    { false Hne1 H6. } *)
+
+    specializes He2 penv0 env.
+    admit.
+
+    (* inverts He2 as.
+    {
+      (* e2 has no shift *)
+      introv Hne2 Hb2.
+      applys sav_base.
+      {
+        introv H1.
+        inverts H1.
+        (* false Hne2 H8. *)
+        applys_eq Hne2. applys_eq H8. f_equal.
+        Fail reflexivity.
+        (* cyclic dependency, we need to know how e2 evaluates to choose shift or no *)
+        (* supply v -> invert He2 -> reason backwards -> supply v *)
+        admit.
+        admit.
+      }
+      admit.
+    }
+    {
+      (* e2 has shift *)
+      introv Hne2 Hb2.
+      admit.
+    } *)
+  }
+  {
+    (* e1 has shift *)
+    introv Hn Hne1 Hb1.
+    applys sav_shift. math.
+    { introv H. inverts H as H1. false Hne1 H1. }
+    { intros.
+      inverts H.
+      { false Hne1 H7. }
+        (* specializes He2 v penv0 env.
+        inverts He2 as. { (* e2 has no shift *) introv Hne2 Hb2. false Hne2 H8. }
+        { (* e2 has shift *)
+          false Hne1 H7. }
+      } *)
+      {
+        (* e1 has a shift *)
+        specializes Hb1 H6.
+        destruct Hb1 as (fb&fk&?&?&?).
+        exs. splits.
+        applys s_bind_sh H.
+        (* intros. *)
+        (* assumption. *)
+        intros. specializes H0 x0.
+        applys_eq H0.
+        f_equal.
+        admit.
+        (* try to use ih *)
+        intros.
+        specializes IH (n-1).
+        forward IH.
+        (* assert (n > 0) as ?. admit. *)
+        unfold downto. math.
+        specializes IH (n1-1) x (ek0 v) e2 (fk v).
+        specializes IH f2.
+        applys IH.
+        admit.
+        math.
+        intros.
+        specializes He2 v0 penv1 env0.
+        admit.
+
+        (* specializes IH. *)
+        (* intros. *)
+        (* eassumption. *)
+        (* specializes IH env. *)
+        (* simpl. case_if. clear C. *)
+        (* assert (x<>x0) as ?. admit. *)
+        (* case_if. clear H2 C. *)
+
+        (* prove the continuation satisfies triple *)
+        (* need the induction hypothesis for ek and e2 *)
+        admit.
+      }
+    }
+  }
+Abort.
+
+Require Import Coq.Program.Equality.
+
+Lemma plet_sound_aux: forall penv env v (ek:val->expr) (fk:val->flow),
+  (forall v, spec_assert_valid_under penv env (ek v) (fk v)) ->
+  spec_assert_valid_under penv env (plet "x" (ek v) (padd (pvar "x") 1))
+    ((fun r1 => let x = fk r1 in (ens (fun r => \[exists i : int, x = i /\ r = i + 1])))
+    v).
+Proof.
+  intros.
+  specializes H v.
+  (* inverts H. *)
+  (* induction H. *)
+  (* dependent induction H. *)
+  induction H using spec_assert_valid_under_ind1.
+  (* remember (ek v) as e. *)
+  (* remember (fk v) as f. *)
+  (* induction H using spec_assert_valid_under_ind1; subst. *)
+  { (* ek has no shift *)
+      applys sav_base.
+      { intros.
+        introv H2.
+        inverts H2.
+        { false_invert H10. }
+        { false H H8. } }
+      intros.
+      inverts H1. simpl in H10.
+      specializes H0 H9.
+      applys s_bind H0.
+
+      inverts H10.
+      injects H8.
+
+      applys s_ens.
+      exs.
+      splits*.
+      hintro.
+      exists i1.
+      splits*.
+      fmap_eq.
+  }
+  {
+    (* ek has shift *)
+    applys sav_shift. { introv H1. inverts H1. false H H9. }
+    intros.
+    inverts H1. { false H H9. } clear H.
+    specializes H0 H8.
+    destr H0.
+    exs.
+    splits.
+    applys s_bind_sh H.
+    {
+      (* clear H2. *)
+      intros x.
+      applys H0 x. clear H0.
+      
+
+      admit.
+    }
+    {
+      (* clear H0. *)
+      intros v1.
+      (* applys H2 v1. *)
+      admit.
+    }
+  }
+
+(* Abort. *)
+Admitted.
+
+Lemma plet_sound_test: forall x e1 e2 f1 (f2:val->flow),
+  spec_assert_valid e1 f1 ->
+  (forall v, spec_assert_valid (subst x v e2) (f2 v)) ->
+  spec_assert_valid (plet x e1 e2) (bind f1 f2).
+Proof.
+  unfold spec_assert_valid. introv He1 He2. intros. specializes He1 penv0 env.
+  assert (x = "x") as ?. admit.
+  assert (e1 = pshift (fun k => papp (pvar k) 1)) as ?. admit.
+  assert (f1 = sh (fun k => unk k 1)) as ?. admit.
+  assert (e2 = padd (pvar "x") 1) as ?. admit.
+  assert (f2 = (fun x => ens (fun r => \[exists i, x = vint i /\ r = i + 1]))) as ?. admit.
+  subst.
+
+  inverts He1.
+  { applys sav_base.
+    { intros. introv H1. inverts H1. false_invert H9. false H H8. }
+    { intros. inverts H1. false_invert H9. } }
+  applys sav_shift. { intros. introv H1. inverts H1. inverts H9. }
+  intros.
+  inverts H1. { false_invert H9. }
+  specializes H0 H8.
+  clear H.
+  destr H0.
+
+  exs. splits.
+
+  - applys s_bind_sh.
+    applys H.
+  
+  - applys H0.
+
+  - 
+    pose proof plet_sound_aux.
+    intros.
+    specializes H1 penv0 env v H2.
+
+    (* specializes H1 fk. *)
+
+
+    (* v H2. *)
+
+
+    (* specializes H1 v. *)
+    (* specializes H1 H0. *)
+
+
+  (* - intros.
+    specializes He2 v penv0 env.
+    simpl in He2.
+    specializes H2 v.
+    
+    (* see whether ek has shift *)
+    inverts H2.
+    {
+      (* ek has no shift *)
+      applys sav_base.
+      { intros.
+        introv H2.
+        inverts H2.
+        { false_invert H13. }
+        { false H1 H11. } }
+      intros.
+      inverts H2.
+      specializes H3 H12.
+      applys s_bind H3.
+
+      simpl in H13.
+      inverts H13.
+      injects H11.
+
+      applys s_ens.
+      exs.
+      splits*.
+      hintro.
+      Set Printing Coercions.
+      exists i1.
+      splits*.
+      fmap_eq.
+    }
+    {
+      (* ek has shift *)
+      applys sav_shift. { introv H2. inverts H2. false H1 H12. }
+      intros.
+      inverts H2.
+      { simpl in H13. inverts H13. }
+      
+      specializes H3 H11.
+      destr H3.
+      exs.
+      splits.
+      applys s_bind_sh.
+      applys H2.
+      assumption.
+      intros.
+      (* induction? *)
+
+      admit.
+    } *)
+Abort.
+
+Lemma plet_sound_test: forall x e1 e2 f1 (f2:val->flow),
+  spec_assert_valid e1 f1 ->
+  (forall v, spec_assert_valid (subst x v e2) (f2 v)) ->
+  spec_assert_valid (plet x e1 e2) (bind f1 f2).
+Proof.
+  unfold spec_assert_valid. introv He1 He2. intros. specializes He1 penv0 env.
+  assert (x = "x") as ?. admit.
+  assert (e1 = 1) as ?. admit.
+  assert (f1 = ens (fun r => \[r = 1])) as ?. admit.
+  assert (e2 = padd (pvar "x") 1) as ?. admit.
+  assert (f2 = (fun x => ens (fun r => \[exists i, x = vint i /\ r = i + 1]))) as ?. admit.
+  subst.
+
+  inverts He1.
+  2: { applys sav_shift. intros. introv H1. inverts H1. false H H9. intros. inverts H1. inverts H10. inverts H8. }
+
+  applys sav_base.
+  { intros. introv H1. inverts H1. inverts H10. inverts H8. }
+  intros.
+  inverts H1.
+  specializes H0 H9.
+  specializes He2 v0 penv0 env.
+  simpl in He2.
+  inverts He2. 2: { false H1 H10. }
+
+  applys s_bind H0.
+  applys* H2.
+
+Abort.
